autosubst proof

stlc/reduction.v
@@ -6,8 +6,11 @@ Inductive value {n : nat} : tm n -> Prop :=
   | v_true : value tmtrue
   | v_false : value tmfalse.
 
+Hint Constructors value : core.
+
 Inductive step {n : nat} : tm n -> tm n -> Prop :=
   | S_β a b A :
+    value b ->
     step (tmapp (tmabs A a) b) (subst_tm (b..) a)
   | ST_App1 e1 e1' e2 :
     step e1 e1' ->
@@ -24,6 +27,81 @@ Inductive step {n : nat} : tm n -> tm n -> Prop :=
     step e1 e1' ->
     step (tmif e1 e2 e3) (tmif e1' e2 e3).
 
+Hint Constructors step : core.
+
 Definition multistep {n : nat} := rtc (@step n).
 
+Hint Unfold multistep : core.
+Hint Constructors rtc : core.
+
 Definition steps {n : nat} (e : tm n) : Prop := exists e', value e' /\ multistep e e'.
+
+Lemma value_no_step {n} : forall (v : tm n),
+    value v ->
+    ~ (exists v', step v v').
+Proof.
+  intros. inversion H; unfold not; intros [v' Hv']; inversion Hv'.
+Qed.
+
+Ltac val_step :=
+  match goal with
+    H1: value ?e,
+    H2: step ?e ?e'
+    |- _ => apply value_no_step in H1; exfalso; apply H1; exists e'; apply H2
+  end.
+
+Lemma determinism {n} : forall (e e1 e2 : tm n),
+    step e e1 ->
+    step e e2 ->
+    e1 = e2.
+Proof.
+  induction e; intros.
+  - inversion H.
+  - inversion H; inversion H0; subst; try val_step.
+    + inversion H5. reflexivity.
+    + inversion H8.
+    + inversion H4.
+    + apply IHe1 with (e2 := e1') in H8; subst; auto.
+    + apply IHe2 with (e1 := e2') in H10; subst; auto.
+  - inversion H.
+  - inversion H.
+  - inversion H.
+  - inversion H; subst.
+    + inversion H0; subst.
+      * reflexivity.
+      * inversion H5.
+    + inversion H0; subst.
+      * reflexivity.
+      * inversion H5.
+    + inversion H0; subst.
+      * inversion H5.
+      * inversion H5.
+      * apply IHe1 with (e2 := e1') in H6; subst; auto.
+Qed.
+
+Lemma multi_if_cong {n : nat} : forall (e1 e2 e3 e1' : tm n),
+    multistep e1 e1' -> multistep (tmif e1 e2 e3) (tmif e1' e2 e3).
+Proof.
+  intros. induction H; eauto.
+Qed.
+
+Hint Resolve multi_if_cong : core.
+
+Lemma multi_app_cong1 {n : nat} : forall (e1 e1' e2 : tm n),
+    multistep e1 e1' ->
+    multistep (tmapp e1 e2) (tmapp e1' e2).
+Proof.
+  intros. induction H; eauto.
+Qed.
+
+Hint Resolve multi_app_cong1 : core.
+
+Lemma multi_app_cong2 {n : nat} : forall (e1 e2 e2' : tm n),
+    value e1 ->
+    multistep e2 e2' ->
+    multistep (tmapp e1 e2) (tmapp e1 e2').
+Proof.
+  intros. induction H0; eauto.
+Qed.
+
+Hint Resolve multi_app_cong2 : core.
