stlc/norm.v
@@ -78,14 +78,10 @@ Lemma N'_backpreservation : forall τ (e e' : tm 0),
     N' τ e' -> N' τ e.
 Proof.
   induction τ; simpl; intros e e' Hty Hstep [Nty [Nstep Nelim]]; repeat split; eauto;
-  try (destruct Nstep as [v [Hval Hstv]]; exists v; split; try assumption;
-    econstructor; eassumption).
+  try (destruct Nstep as [v [Hval Hstv]]; exists v; split; try assumption; econstructor; eassumption).
   intros. specialize Nelim with e'0. remember H. clear Heqn. apply Nelim in H.
-  assert (step (tmapp e e'0) (tmapp e' e'0)). { constructor. assumption. }
-  apply IHτ2 with (e' := tmapp e' e'0); try assumption.
-  econstructor.
-    * apply Hty.
-    * apply N'_implies_typed. assumption.
+  assert (step (tmapp e e'0) (tmapp e' e'0)) by auto.
+  apply IHτ2 with (e' := tmapp e' e'0); eauto using N'_implies_typed.
 Qed.
 
 Lemma N'_multi_backpreservation : forall τ (e e' : tm 0),
@@ -98,28 +94,6 @@ Proof.
   - apply IHrtc in H1.
     + eapply N'_backpreservation; eassumption.
     + eapply preservation; eassumption.
-Qed.
-
-Lemma multi_if_cong {n : nat} : forall (e1 e2 e3 e1' : tm n),
-    multistep e1 e1' -> multistep (tmif e1 e2 e3) (tmif e1' e2 e3).
-Proof.
-  intros. induction H.
-  - constructor.
-  - econstructor.
-    + constructor. eassumption.
-    + assumption.
-Qed.
-
-Lemma multi_app_cong2 {n : nat} : forall (e1 e2 e2' : tm n),
-    value e1 ->
-    multistep e2 e2' ->
-    multistep (tmapp e1 e2) (tmapp e1 e2').
-Proof.
-  intros. induction H0.
-  - constructor.
-  - econstructor.
-    + apply ST_App2; eassumption.
-    + assumption.
 Qed.
 
 Lemma γ_ok'_impl_good_subst {n : nat} : forall γ (Γ : context n),
@@ -138,9 +112,7 @@ Proof.
   intros Γ γ e τ Hty. induction Hty; subst; intros Hγ.
   - (* var *) simpl. unfold γ_ok' in Hγ. specialize Hγ with i. apply Hγ.
   - (* abs *) repeat split.
-    + eapply morphing.
-      * constructor. eassumption.
-      * apply γ_ok'_impl_good_subst. assumption.
+    + eapply morphing; eauto using γ_ok'_impl_good_subst.
     + exists (subst_tm γ (tmabs τ1 e)). split; constructor.
     + intros. simpl. remember H. clear Heqn0. apply N'_implies_norm in H. destruct H as [v [Hval Hstepv]].
       eapply N'_multi_backpreservation.
@@ -150,10 +122,8 @@ Proof.
            ++ apply γ_ok'_impl_good_subst in Hγ. apply good_subst_ext. assumption.
         -- apply N'_implies_typed in n0. apply n0.
       * eapply rtc_r.
-        -- apply multi_app_cong2.
-           ++ constructor.
-           ++ eassumption.
-        -- apply S_β.
+        -- apply multi_app_cong2; eauto.
+        -- apply S_β. assumption.
       * asimpl. apply IHHty. apply γ_ok'_cons.
         -- eapply N'_multi_preservation; eassumption.
         -- assumption.
@@ -183,7 +153,7 @@ Qed.
 
 Fixpoint N (τ : ty) (e : tm 0) : Prop :=
   match τ with
-    | tybool => (multistep e tmtrue \/ multistep e tmfalse)
+    | tybool => multistep e tmtrue \/ multistep e tmfalse
     | tyarr τ1 τ2 => forall e', N τ1 e' -> N τ2 (tmapp e e')
   end.
 
@@ -200,17 +170,118 @@ Fixpoint N (τ : ty) (e : tm 0) : Prop :=
 (*       * assumption. *)
 (*       * constructor. *)
 
+(* Lemma app_step_abs {n} : forall (e1 e2 : tm n), *)
+(*     steps (tmapp e1 e2) -> *)
+(*     exists τ e, multistep e1 (tmabs τ e). *)
+(* Proof. *)
+(*   intros. destruct H as [v [Hval Hstep]]. *)
+(*   inversion Hstep; subst. *)
+(*   - inversion Hval. *)
+(*   - inversion H; subst. *)
+(*     + exists A, a. constructor. *)
+(*     +  *)
+
 Lemma N_implies_norm : forall τ e,
     N τ e -> steps e.
 Proof.
   induction τ.
-  - (* -> *) intros. simpl in H. eapply IHτ2 in H.
+  - (* -> *) intros. simpl in H. induction τ1.
+    + admit.
+    + specialize H with tmtrue. apply IHτ2 in H.
+      * inversion H.
+    eapply IHτ2 in H.
     + admit.
     + admit.
   - (* bool *) intros. simpl in H. destruct H.
-    + exists tmtrue. split.
+    + exists tmtrue. split; auto.
+    + exists tmfalse. split; auto.
+Admitted.
+
+(* don't check domain equality bc both total functions over fin n *)
+Definition γ_ok {n : nat} (γ : fin n -> tm 0) (Γ : context n) :=
+  forall i, N (Γ i) (γ i).
+
+Lemma γ_ok_cons {n} {γ : fin n -> tm 0} {Γ a A} :
+  N A a ->
+  γ_ok γ Γ ->
+  γ_ok (a .: γ) (A .: Γ).
+Proof.
+  unfold γ_ok.
+  intros h hγ [i|]; simpl; eauto.
+Qed.
+
+Lemma N_backpreservation : forall τ (e e' : tm 0),
+    step e e' ->
+    N τ e' -> N τ e.
+Proof.
+  induction τ.
+  - (* -> *) simpl. intros. eapply IHτ2; eauto using ST_App1.
+  - (* bool *) simpl. intros. destruct H0.
+    + left. eauto.
+    + right. eauto.
+Qed.
+
+Lemma N_multi_backpreservation : forall τ (e e' : tm 0),
+    multistep e e' ->
+    N τ e' -> N τ e.
+Proof.
+  intros. induction H; eauto using N_backpreservation.
+Qed.
+
+Lemma N_preservation : forall τ (e e' : tm 0),
+    step e e' ->
+    N τ e -> N τ e'.
+Proof.
+  induction τ.
+  - (* -> *) simpl. intros. eapply IHτ2.
+    + constructor. eassumption.
+    + apply H0. assumption.
+  - (* bool *) intros. simpl. destruct H0.
+    + left. inversion H0; subst.
+      * inversion H.
+      * apply determinism with (e1 := y) in H; subst; assumption.
+    + right. inversion H0; subst.
+      * inversion H.
+      * apply determinism with (e1 := y) in H; subst; assumption.
+Qed.
+
+Lemma N_multi_preservation : forall τ (e e' : tm 0),
+    multistep e e' ->
+    N τ e -> N τ e'.
+Proof.
+  intros. induction H; eauto using N_preservation.
+Qed.
+
+Lemma fundamental_lemma : forall Γ γ (e : tm 0) τ,
+    has_type Γ e τ ->
+    γ_ok γ Γ ->
+    N τ (subst_tm γ e).
+Proof.
+  intros Γ γ e τ Hty Hγ. induction Hty.
+  - (* var *) simpl. subst. apply Hγ.
+  - (* abs *) simpl. intros. remember H. clear Heqn0.
+    apply N_implies_norm in H. destruct H as [v [Hval Hstep]].
+    eapply N_multi_backpreservation.
+    + eapply rtc_r.
+      * apply multi_app_cong2.
+        -- constructor.
+        -- eassumption.
       * constructor.
-      * assumption.
-    + exists tmfalse. split.
-      * constructor.
-      * assumption.
+    + asimpl. apply IHHty. apply γ_ok_cons; eauto using N_multi_preservation.
+  - (* app *) simpl. specialize IHHty1 with γ. remember Hγ. clear Heqγ0.
+    apply IHHty1 in Hγ. simpl in Hγ.
+    specialize Hγ with (subst_tm γ e2). apply Hγ. apply IHHty2. assumption.
+  - (* true *) simpl. left. constructor.
+  - (* false *) simpl. right. constructor.
+  - (* if *) simpl. remember Hγ. clear Heqγ0. apply IHHty1 in Hγ. destruct Hγ.
+    + apply N_multi_backpreservation with (e' := subst_tm γ e2).
+      * eapply rtc_r.
+        -- apply multi_if_cong. eassumption.
+        -- constructor.
+      * apply IHHty2. assumption.
+    + apply N_multi_backpreservation with (e' := subst_tm γ e3).
+      * eapply rtc_r.
+        -- apply multi_if_cong. eassumption.
+        -- constructor.
+      * apply IHHty3. assumption.
+Qed.
