stlc/safety.v
@@ -1,0 +1,86 @@
+Require Export typing.
+Require Export reduction.
+Require Export stlc.
+
+From stdpp Require Import relations.
+
+Inductive V : ty -> tm 0 -> Prop :=
+  | V_True : V tybool tmtrue
+  | V_False : V tybool tmfalse
+  | V_Arr e τ1 τ2 : (forall v, V τ1 v -> E τ2 (subst_tm v.. e)) ->
+                    V (tyarr τ1 τ2) (tmabs τ1 e)
+with E : ty -> tm 0 -> Prop :=
+  | E_St e τ : (forall e', (multistep e e' /\ ~ exists e'', step e' e'') -> V τ e') ->
+               E τ e.
+
+Hint Constructors V : core.
+Hint Constructors E : core.
+
+Definition γ_ok {n} (γ : fin n -> tm 0) (Γ : context n) : Prop :=
+  forall x, V (Γ x) (γ x).
+
+(* Lemma V_backpreservation : forall τ e e', *)
+(*     step e e' -> V τ e' -> V τ e. *)
+(* Proof. *)
+(*   induction τ; intros. *)
+(*   - (* -> *) inversion H0. inversion H6. subst. *)
+
+Lemma V_val : forall τ v,
+    V τ v -> value v.
+Proof.
+  induction τ; intros; inversion H; constructor.
+Qed.
+
+
+Lemma V_no_step : forall τ e,
+    V τ e -> ~ exists e', step e e'.
+Proof.
+  induction τ; unfold not; intros.
+  - (* -> *) inversion H. subst. destruct H0. inversion H0.
+  - (* bool *) destruct H0. inversion H; subst; inversion H0.
+Qed.
+
+Lemma V_impl_E : forall τ e,
+    V τ e -> E τ e.
+Proof.
+  intros. apply E_St with (e' := e).
+  - split; eauto using V_no_step.
+  - assumption.
+Qed.
+
+Lemma fundamental_lemma : forall (e : tm 0) τ γ Γ,
+    has_type Γ e τ ->
+    γ_ok γ Γ ->
+    E τ (subst_tm γ e).
+Proof.
+  intros e τ γ Γ Hty Hγ. induction Hty.
+  - (* var *) simpl. subst. apply V_impl_E. apply Hγ.
+  - (* abs *) simpl. admit.
+  - (* app *) simpl. remember Hγ. clear Heqγ0. apply IHHty1 in γ0.
+    remember Hγ. clear Heqγ1. apply IHHty2 in γ1.
+    inversion γ0. inversion γ1. inversion H0. subst.
+    destruct H as [Hste1 Hirre1]. destruct H3 as [Hste2 Hirre2].
+    econstructor.
+    + split.
+      * apply rtc_transitive with (y := tmapp (tmabs τ1 e3) e'0).
+        -- apply rtc_transitive with (y := tmapp (tmabs τ1 e3) (subst_tm γ e2)).
+           ++ apply multi_app_cong1. assumption.
+           ++ apply multi_app_cong2; auto.
+        -- apply rtc_transitive with (y := subst_tm e'0.. e3).
+           ++ econstructor.
+              ** constructor. eapply V_val. eassumption.
+              ** constructor.
+           ++ inversion H11. destruct H as [Hst _]. apply Hst.
+    apply E_St with (e' := subst_tm e'0.. e3).
+    + destruct H as [Hste1 Hirre1]. destruct H3 as [Hste2 Hirre2]. split.
+      * apply rtc_transitive with (y := tmapp (tmabs τ1 e3) e'0).
+        -- apply rtc_transitive with (y := tmapp (tmabs τ1 e3) (subst_tm γ e2)).
+           ++ apply multi_app_cong1. assumption.
+           ++ apply multi_app_cong2; auto.
+        -- econstructor.
+           ++ constructor. eapply V_val. eassumption.
+           ++ constructor.
+      *
+  - (* if *) simpl. remember Hγ. clear Heqγ0.
+    apply IHHty1 in γ0. inversion γ0.
+    + constructor.
